prove the very first Coq-verified iris Hoare Triple :)

barrier/tests.v
@@ -1,25 +1,25 @@
 (** This file is essentially a bunch of testcases. *)
-Require Import modures.base.
-Require Import barrier.parameter.
+Require Import modures.logic.
+Require Import barrier.lifting.
+Import uPred.
 
 Module LangTests.
-  Definition add := Op2 plus (Lit 21) (Lit 21).
-
-  Goal ∀ σ, prim_step add σ (Lit 42) σ None.
+  Definition add :=  Plus (LitNat 21) (LitNat 21).
+  Goal ∀ σ, prim_step add σ (LitNat 42) σ None.
   Proof.
-    apply Op2S.
+    constructor.
   Qed.
 
   Definition rec := Rec (App (Var 0) (Var 1)). (* fix f x => f x *)
-  Definition rec_app := App rec (Lit 0).
+  Definition rec_app := App rec (LitNat 0).
   Goal ∀ σ, prim_step rec_app σ rec_app σ None.
   Proof.
     move=>?. eapply BetaS.
     reflexivity.
   Qed.
 
-  Definition lam := Lam (Op2 plus (Var 0) (Lit 21)).
-  Goal ∀ σ, prim_step (App lam (Lit 21)) σ add σ None.
+  Definition lam := Lam (Plus (Var 0) (LitNat 21)).
+  Goal ∀ σ, prim_step (App lam (LitNat 21)) σ add σ None.
   Proof.
     move=>?. eapply BetaS. reflexivity.
   Qed.
@@ -28,3 +28,34 @@ End LangTests.
 Module ParamTests.
   Print Assumptions Σ.
 End ParamTests.
+
+Module LiftingTests.
+  (* TODO RJ: Some syntactic sugar for language expressions would be nice. *)
+  Definition e3 := Load (Var 0).
+  Definition e2 := Seq (Store (Var 0) (Plus (Load (Var 0)) (LitNat 1))) e3.
+  Definition e := Let (Alloc (LitNat 1)) e2.
+  Goal ∀ σ E, (ownP (Σ:=Σ) σ) ⊑ (wp (Σ:=Σ) E e (λ v, ■(v = LitNatV 2))).
+  Proof.
+    move=> σ E. rewrite /e.
+    rewrite -(wp_bind _ _ (LetCtx EmptyCtx e2)). rewrite -wp_mono.
+    { eapply wp_alloc; done. }
+    move=>v; apply exist_elim=>l. apply const_elim_l; move=>[-> _] {v}.
+    rewrite (later_intro (ownP _)); apply wp_lam. asimpl.
+    rewrite -(wp_bind _ _ (SeqCtx (StoreRCtx (LocV _)
+                                   (PlusLCtx EmptyCtx _)) (Load (Loc _)))).
+    rewrite -wp_mono.
+    { eapply wp_load. apply: lookup_insert. } (* RJ TODO: figure out why apply and eapply fail. *)
+    move=>v; apply const_elim_l; move=>-> {v}.
+    rewrite -(wp_bind _ _ (SeqCtx (StoreRCtx (LocV _) EmptyCtx) (Load (Loc _)))).
+    rewrite (later_intro (ownP _)); apply wp_plus.
+    rewrite -(wp_bind _ _ (SeqCtx EmptyCtx (Load (Loc _)))).
+    rewrite -wp_mono.
+    { eapply wp_store; first reflexivity. apply: lookup_insert. }
+    move=>v; apply const_elim_l; move=>-> {v}.
+    rewrite (later_intro (ownP _)); apply wp_lam. asimpl.
+    rewrite -wp_mono.
+    { eapply wp_load. apply: lookup_insert. }
+    move=>v; apply const_elim_l; move=>-> {v}.
+    by apply const_intro.
+  Qed.
+End LiftingTests.
